* Updates LTS definitions, added documentation

src/formalisms/lts.v
@@ -29,66 +29,187 @@
  *
  * DM21-0762
 ***)
-(** %\chapter{Labelled Transitionsition System (LTS)}\label{chap::lts}%
+(*|
 
-In this chapter, we define Labelled Transition Systems (or LTS). This definition follows the canonical definition of a _deterministic_ LTS, see %\cite00{gorrieriLabeledTransitionSystems2017a}%. *)
+**************************************
+Labelled Transitionsition System (LTS)
+**************************************
 
-(* begin hide *)
+In this chapter, we define Labelled Transition Systems (or LTS). This definition
+follows the canonical definition of a *deterministic* LTS, see :math:`\cite{gorrieriLabeledTransitionSystems2017a}` for details. |*)
+
+(*| .. coq:: none |*)
 Require Import Coq.Lists.List.
 Import ListNotations. (* from List *)
+Require Import Coq.Relations.Relation_Definitions.
+Require Import Coq.Classes.RelationClasses.
 
 Section LTS_Definition.
-(* end hide *)
+(*| .. coq:: no-out |*)
 
-(** * Definition of LTS
+(*|
 
-_Notes_:
-- we opted for [bool] rather than [Prop] to allow for on-the-fly evaluation of the LTS.
-- we define both a [LTS_Transition] predicate and a [LTS_Step] function. The step function allows building a simulator, whereas the transition function allows performing proof. We keep the definition of [LTS_Transition] but are likely to remove it ultimately.
+===================
+Definition of a LTS
+===================
 
-*)
+ A labeled transition system (or LTS) is a triple LTS = (S, A, Step) where
 
-  Definition LTS_Transitions (S : Type) (A : Type) := S -> A -> S -> bool.
+* S is the nonempty, countable set of states
+* A is the countable set of labels (or actions);
+* Step : S x A x S is the transition relation.
+
+*Note*: we define :coq:`LTS_Step` as a function rather than a proposition. The :coq:`Step` function allows building a simulator, whereas the relation supports only proof.
+
+|*)
 
   Definition LTS_Step (S : Type) (A : Type) := S -> A -> S.
 
-  Record LTS_struct : Type := mkLTS_struct  {
+  Record LTS_struct : Type := mkLTS_struct {
     States : Type;
-    Init : States;
     Actions : Type;
-    Steps : LTS_Step States Actions;
+    Step : LTS_Step States Actions;
+    Init : States;
   }.
 
-(** [step_lts] performs one step of the LTS. *)
+(*| :coq:`step_lts` performs one step of the LTS. |*)
 
-  Definition step_lts
-    (A_LTS : LTS_struct) (state: States A_LTS) (action : Actions A_LTS) :=
-      (Steps A_LTS) state action.
+  Definition step_lts (A_LTS : LTS_struct)
+                      (state: States A_LTS)
+                      (action : Actions A_LTS) :=
+    (Step A_LTS) state action.
 
-(** See implementation in [lts.v] for example of use. *)
+(*| .. coq:: none |*)
+Section LTS_Properties.
+(*| .. coq:: no-out |*)
 
-(* begin hide *)
+(*|
+
+===================
+Properties of a LTS
+===================
+
+We define :coq:`Transitions` as a predicate that returns
+:coq:`True` iff :math:`s \xrightarrow{\text{a}} s'`.
+
+|*)
+
+Definition Transitions
+  (L : LTS_struct) (s : States L) (a : Actions L) (s' : States L) :=
+  (Step L) s a = s'.
+
+(*| :coq:`Reachable` is a predicate that evaluates to True if a state is reachable from s. We use an inductive definition to defines this predicate with the following two case: either s is accessible from s, else if s1 is accessible from s and a transition from s1 to s2 exists, then s2 is also accessible from s.
+|*)
+
+Inductive Reachable (L : LTS_struct) (s : States L) :
+  States L -> Prop :=
+  | reachable_default : Reachable L s s
+  | reachable_step :
+      forall (s1 s2 : States L) (t : Actions L),
+      Reachable L s s1 -> Transitions L s1 t s2
+      -> Reachable L s s2.
+
+(*| :coq:`Deadlock` returns True if s1 is a deadlock state, i.e. there is no transition from s1. |*)
+
+Definition Deadlock (L : LTS_struct) (s1 : States L) : Prop :=
+  forall (t : Actions L) (s2 : States L), ~ Transitions L s1 t s2.
+
+(*| Definition of a :coq:`Bisimulation` relation. |*)
+
+Definition Bisimulation (L : LTS_struct)
+                        (R : relation (States L)) : Prop :=
+  forall p q : States L, R p q ->
+  (forall (a : Actions L) (p' : States L), Transitions L p a p' ->
+    exists2 q' : States L, Transitions L q a q' & R p' q') /\
+  (forall (a : Actions L) (q' : States L), Transitions L q a q' ->
+    exists2 p' : States L, Transitions L p a p' & R p' q').
+
+(*| Two States are bisimilar when a bisimulation exists. |*)
+
+Inductive Bisimilar (L : LTS_struct) (p q : States L) : Prop :=
+    bisimilar_exist :
+      forall R : relation (States L),
+      R p q -> Bisimulation L R -> Bisimilar L p q.
+
+(*| .. coq:: none |*)
+Section Results.
+
+Variable L : LTS_struct.
+
+Lemma Bisimilar_Refl : reflexive (States L) (Bisimilar L).
+Proof.
+  intros.
+
+  (* To prove this lemma, we build a trivial bisimulation relation: the identity. *)
+  exists (fun (p q : States L) => p = q). trivial.
+  split; intros.
+
+  (* From there, we exhibit a solution for each existential statement*)
+  - exists p'; trivial. rewrite <- H; trivial.
+  - exists q'; trivial. rewrite H; trivial.
+Qed.
+
+Lemma Bisimilar_Sym : symmetric (States L) (Bisimilar L).
+Proof.
+  (* introduce all variables *)
+  unfold symmetric.
+  intros ; elim H; intros.
+
+  (* To prove this lemma, we propose the R' relation, which
+    is the symetric of R and reduce all terms *)
+  exists (fun p q : States L => R q p); trivial.
+  red in |- *; intros.
+
+  (* We can now combine H1 and H2 to conclude *)
+  elim H1 with (1 := H2); auto.
+Qed.
+
+Lemma Bisimilar_Trans : transitive (States L) (Bisimilar L).
+Proof.
+  unfold transitive.
+
+  (* introduce all variable. We turn Bisimilar predicates into Bisimulation *)
+  intros p q r H1 H2. case H1. case H2. clear H1 H2. intros.
+
+  (* the previous steps introduced relations R0 between p and q, and R between
+     q and r. We use them to build a new relation that relates p and r*)
+  exists (fun p r : States L => exists2 q : States L, R0 p q & R q r).
+  - exists q; auto.
+  - red in |- *; intros.
+
+    (* from that point, the game is to break all quantifiers and exhibit
+    solutions *)
+    case H3; clear H3; intros.
+    case H2 with (1 := H3); clear H2; intros.
+    case H0 with (1 := H4); clear H0; intros.
+    split; intros.
+    * case H2 with (1 := H7); clear H2; intros.
+      case H0 with (1 := H2); clear H0; intros.
+      exists x1; trivial; exists x0; trivial.
+    * case H6 with (1 := H7); clear H6; intros.
+      case H5 with (1 := H6); clear H5; intros.
+      exists x1; trivial; exists x0; trivial.
+Qed.
+(*| .. coq::  |*)
+
+(*|
+:coq:`Bisimilar` is an equivalence relation.
+|*)
+
+Instance Bisimilar_Equivalence : Equivalence (Bisimilar L) := {|
+  Equivalence_Reflexive := Bisimilar_Refl;
+  Equivalence_Symmetric := Bisimilar_Sym ;
+  Equivalence_Transitive := Bisimilar_Trans ;
+|}.
+
+(*| .. coq:: none |*)
+End Results.
+
+End LTS_Properties.
+
 End LTS_Definition.
 
-(* The following could be added to the definition of a LTS *)
- (* Transitions : LTS_Transitions States Actions;
-
- XXX But this seems like an unnecessary definition
- *)
-
-(*
-Definition Transitions_Steps_Equivalent (A_LTS : LTS_struct) :=
-  forall (state: States A_LTS) (action: Actions A_LTS),
-  exists x: (States A_LTS), In x ((Steps A_LTS) state action) ->
-    (Transitions A_LTS state action x) = true.
-
-Definition step_lts_predicate
-  (A_LTS : LTS_struct) (current_state : States A_LTS)
-  (action : Actions A_LTS) (destination : States A_LTS) :=
-    (Transitions A_LTS) current_state action destination.
-*)
-
-(** Example *)
+(* Example *)
 
 Section Example.
 
@@ -112,25 +233,24 @@ Definition LTS_Test : LTS_struct := {|
   States := ab;
   Init := A;
   Actions := ab_actions;
-  (*Transitions := AB_Transitions; *)
-  Steps := AB_Steps;
+  Step := AB_Steps;
 |}.
 
-(*
-Lemma e: Transitions_Steps_Equivalent LTS_Test.
-Proof.
-    unfold Transitions_Steps_Equivalent.
-    intros.
-    induction state.
-    - now exists B.
-    - now exists A.
-Qed.
-*)
 Example f' := step_lts LTS_Test (Init LTS_Test) ReadA.
 Lemma test : f' = B.
 Proof.
   auto.
 Qed.
 
+Example LTS_Test_All_Reachable : forall s : ab, Reachable LTS_Test A s.
+Proof.
+  intros.
+  induction s.
+  - apply reachable_default.
+  - apply reachable_step with (s1 := A) (t := ReadA).
+    * apply reachable_default.
+    * unfold Transitions; auto.
+Qed.
+
 End Example.
-(* end hide *)
+(*| .. coq:: |*)
